open import Variables

open import Data.Bool
open import Data.List using (List; []; _∷_)
open import Data.Nat using (ℕ; zero; suc; _+_)
open import Data.Nat.Properties
open import Function using (_∘_)
import Relation.Binary.PropositionalEquality as Eq
open Eq using (_≡_; refl; sym; cong; cong₂; cong-app)
open Eq.≡-Reasoning using (begin_; _≡⟨⟩_; _≡⟨_⟩_; _∎)
open import Relation.Nullary using (¬_)


module Syntax3 (Op : Set) (sig : Op → List ℕ) where

data Args (Γ : ℕ) : (sig : List ℕ) → Set

data AST : ℕ → Set where

  `_ : ∀{Γ} → (x : Var Γ) → AST Γ

  _⦅_⦆ : ∀{Γ} → (op : Op) → Args Γ (sig op) → AST Γ


data Arg  (Γ : ℕ) : (sig : ℕ) → Set where
  ast : AST Γ → Arg Γ 0
  bind : ∀{n} → Arg (suc Γ) n → Arg Γ (suc n)

data Args Γ where
  nil : Args Γ []
  cons : ∀{n bs} → Arg Γ n → Args Γ bs → Args Γ (n ∷ bs)

bind-arg : ∀{Γ m} → (n : ℕ) → Arg (n + Γ) m → Arg Γ (n + m)
bind-arg {Γ} zero A = A
bind-arg {Γ}{m} (suc n) A
    with bind-arg {Γ}{suc m} n (bind A)
... | ih rewrite +-suc n m = ih

bind-ast : ∀{Γ} → (n : ℕ) → AST (n + Γ) → Arg Γ n
bind-ast {Γ} n M
    with bind-arg n (ast M)
... | A rewrite +-identityʳ n = A


Subst : ℕ → ℕ → Set
Subst Γ Δ = Var Γ → AST Δ

rename : ∀ {Γ Δ}
     → Rename Γ  Δ
       -------------
     → AST Γ → AST Δ
rename-arg : ∀ {Γ Δ n}
     → Rename Γ  Δ
       -----------------
     → Arg Γ n → Arg Δ n
renames : ∀ {Γ Δ S}
      → Rename Γ Δ
        -------------------
      → Args Γ S → Args Δ S

rename ρ (` x)          =  ` (ρ x)
rename ρ (o ⦅ As ⦆)     =  o ⦅ renames ρ As ⦆
rename-arg ρ (ast M)    =  ast (rename ρ M)
rename-arg ρ (bind A)   = bind (rename-arg (ext ρ) A)
renames ρ nil           = nil
renames ρ (cons A As) = cons (rename-arg ρ A) (renames ρ As)

exts : ∀ {Γ Δ}
   → Subst Γ Δ
     ----------------------
   → Subst (suc Γ) (suc Δ)
exts σ Z      =  ` Z
exts σ (S x)  =  rename S_ (σ x)

⟪_⟫ : ∀ {Γ Δ}
  → Subst Γ Δ
    -------------
  → AST Γ → AST Δ
subst-arg : ∀ {Γ Δ n}
  → Subst Γ Δ
    -----------------
  → Arg Γ n → Arg Δ n
substs : ∀ {Γ Δ S}
  → Subst Γ Δ
    -------------------
  → Args Γ S → Args Δ S

⟪ σ ⟫ (` x)          =  σ x
⟪ σ ⟫ (o ⦅ Ms ⦆)     =  o ⦅ substs σ Ms ⦆
subst-arg σ (ast M)  = ast (⟪ σ ⟫ M)
subst-arg σ (bind M) = bind (subst-arg (exts σ) M)
substs σ nil         = nil
substs σ (cons M Ms) = cons (subst-arg σ M) (substs σ Ms)

subst-zero : ∀ {Γ} → (AST Γ) → Var (suc Γ) → (AST Γ)
subst-zero M Z      = M
subst-zero M (S x)  = ` x

_[_] : ∀ {Γ}
   → AST (suc Γ)
   → AST Γ
     ---------
   → AST Γ
_[_] N M =  ⟪ subst-zero M ⟫ N

ids : ∀{Γ} → Subst Γ Γ
ids {Γ} x = ` x

↑ : ∀{Γ} → Subst Γ (suc Γ)
↑ x = ` (S x)

infixr 6 _•_
_•_ : ∀{Γ Δ} → (AST Δ) → Subst Γ Δ → Subst (suc Γ) Δ
(M • σ) Z = M
(M • σ) (S x) = σ x


infixr 5 _⨟_
_⨟_ : ∀{Γ Δ Σ} → Subst Γ Δ → Subst Δ Σ → Subst Γ Σ
σ ⨟ τ = ⟪ τ ⟫ ∘ σ


ren : ∀{Γ Δ} → Rename Γ Δ → Subst Γ Δ
ren ρ = ids ∘ ρ


sub-head : ∀ {Γ Δ} {M : AST Δ}{σ : Subst Γ Δ}
         → ⟪ M • σ ⟫ (` Z) ≡ M
sub-head = refl


sub-tail : ∀{Γ Δ} {M : AST Δ} {σ : Subst Γ Δ}
         → (↑ ⨟ M • σ) ≡ σ
sub-tail = extensionality λ x → refl

sub-η : ∀{Γ Δ} {σ : Subst (suc Γ) Δ} 
      → (⟪ σ ⟫ (` Z) • (↑ ⨟ σ)) ≡ σ
sub-η {Γ}{Δ}{σ} = extensionality λ x → lemma
   where 
   lemma : ∀ {x} → ((⟪ σ ⟫ (` Z)) • (↑ ⨟ σ)) x ≡ σ x
   lemma {x = Z} = refl
   lemma {x = S x} = refl


Z-shift : ∀{Γ}
        → ((` Z) • ↑) ≡ ids
Z-shift {Γ} = extensionality lemma 
   where
   lemma : (x : Var (suc Γ)) → ((` Z) • ↑) x ≡ ids x
   lemma Z = refl
   lemma (S y) = refl

sub-idL : ∀{Γ Δ} {σ : Subst Γ Δ}
       → ids ⨟ σ ≡ σ
sub-idL = extensionality λ x → refl

sub-dist :  ∀{Γ Δ Σ} {σ : Subst Γ Δ} {τ : Subst Δ Σ} {M : AST Δ}
         → ((M • σ) ⨟ τ) ≡ ((⟪ τ ⟫ M) • (σ ⨟ τ))
sub-dist {Γ}{Δ}{Σ}{σ}{τ}{M} = extensionality λ x → lemma {x = x}
  where
  lemma : ∀ {x : Var (suc Γ)} → ((M • σ) ⨟ τ) x ≡ ((⟪ τ ⟫ M) • (σ ⨟ τ)) x
  lemma {x = Z} = refl
  lemma {x = S x} = refl

sub-op : ∀{Γ Δ} {σ : Subst Γ Δ} {o : Op}{Ms : Args Γ (sig o)}
        → ⟪ σ ⟫ (o ⦅ Ms ⦆)  ≡ o ⦅ substs σ Ms ⦆
sub-op = refl        


ren-ext : ∀ {Γ Δ} {ρ : Rename Γ Δ}
        → ren (ext ρ) ≡ exts (ren ρ)
ren-ext {Γ}{Δ}{ρ} = extensionality λ x → lemma {x = x}
  where
  lemma : ∀ {x : Var (suc Γ)} → (ren (ext ρ)) x ≡ exts (ren ρ) x
  lemma {x = Z} = refl
  lemma {x = S x} = refl

rename-subst-ren : ∀ {Γ Δ} {ρ : Rename Γ Δ}{M : AST Γ}
                 → rename ρ M ≡ ⟪ ren ρ ⟫ M
renames-subst-ren : ∀ {Γ Δ} {ρ : Rename Γ Δ}{S}{Ms : Args Γ S}
                 → renames ρ Ms ≡ substs (ren ρ) Ms
rename-arg-subst-ren : ∀ {Γ Δ} {ρ : Rename Γ Δ}{n}{A : Arg Γ n}
                 → rename-arg ρ A ≡ subst-arg (ren ρ) A
                 
rename-subst-ren {M = ` x} = refl
rename-subst-ren{Γ}{Δ}{ρ}{o ⦅ Ms ⦆} =
  cong (_⦅_⦆ o) (renames-subst-ren {Ms = Ms})
  
renames-subst-ren {Ms = nil} = refl
renames-subst-ren {ρ = ρ}{Ms = cons M Ms} =
  cong₂ cons (rename-arg-subst-ren{A = M}) (renames-subst-ren{Ms = Ms})

rename-arg-subst-ren {ρ = ρ} {0} {ast M} = cong ast (rename-subst-ren{ρ = ρ}{M})
rename-arg-subst-ren {Γ}{Δ}{ρ} {suc n} {bind A} =
  let ih = rename-arg-subst-ren {ρ = ext ρ}{n}{A} in
  begin
      bind (rename-arg (ext ρ) A)
    ≡⟨ cong bind ih ⟩
      bind (subst-arg (ren (ext ρ)) A)
    ≡⟨ cong bind (cong₂ subst-arg ren-ext refl) ⟩
      bind (subst-arg (exts (ren ρ)) A)
  ∎

ren-shift : ∀{Γ}
          → ren S_ ≡ ↑ 
ren-shift {Γ} = extensionality λ x → lemma {x = x}
  where
  lemma : ∀ {x : Var Γ} → ren (S_) x ≡ ↑ x
  lemma {x = Z} = refl
  lemma {x = S x} = refl

rename-shift : ∀{Γ} {M : AST Γ}
             → rename (S_) M ≡ ⟪ ↑ ⟫ M
rename-shift{Γ}{M} =
  begin
    rename S_ M
  ≡⟨ rename-subst-ren ⟩
    ⟪ ren S_ ⟫ M
  ≡⟨ cong-app (cong ⟪_⟫ ren-shift) M ⟩
    ⟪ ↑ ⟫ M
  ∎

exts-cons-shift : ∀{Γ Δ} {σ : Subst Γ Δ}
                → exts σ ≡ (` Z • (σ ⨟ ↑))
exts-cons-shift = extensionality λ x → lemma{x = x}
  where
  lemma : ∀{Γ Δ} {σ : Subst Γ Δ} {x : Var (suc Γ)}
                  → exts σ x ≡ (` Z • (σ ⨟ ↑)) x
  lemma {x = Z} = refl
  lemma {x = S y} = rename-subst-ren

ext-cons-Z-shift : ∀{Γ Δ} {ρ : Rename Γ Δ}
                 → ren (ext ρ) ≡ (` Z • (ren ρ ⨟ ↑))
ext-cons-Z-shift {Γ}{Δ}{ρ} =
  begin
    ren (ext ρ)
  ≡⟨ ren-ext ⟩
    exts (ren ρ)
  ≡⟨ exts-cons-shift{σ = ren ρ} ⟩
   ((` Z) • (ren ρ ⨟ ↑))
  ∎

subst-Z-cons-ids : ∀{Γ}{M : AST Γ}
                 → subst-zero M ≡ (M • ids)
subst-Z-cons-ids = extensionality λ x → lemma {x = x}
  where
  lemma : ∀{Γ}{M : AST Γ}{x : Var (suc Γ)}
                      → subst-zero M x ≡ (M • ids) x
  lemma {x = Z} = refl
  lemma {x = S x} = refl

exts-ids : ∀{Γ}
         → exts ids ≡ ids
exts-ids {Γ} = extensionality lemma
  where lemma : (x : Var (suc Γ)) → exts ids x ≡ ids x
        lemma Z = refl
        lemma (S x) = refl

sub-id : ∀{Γ} {M : AST Γ}
         → ⟪ ids ⟫ M ≡ M
sub-arg-id : ∀{Γ}{n} {A : Arg Γ n}
         → subst-arg ids A ≡ A
subs-id : ∀{Γ}{S} {Ms : Args Γ S}
         → substs ids Ms ≡ Ms
sub-id {M = ` x} = refl
sub-id {M = o ⦅ Ms ⦆} = cong (_⦅_⦆ o) (subs-id {Ms = Ms})

subs-id {Ms = nil} = refl
subs-id {Ms = cons M Ms} = cong₂ cons sub-arg-id subs-id

sub-arg-id {A = ast M} = cong ast (sub-id{M = M})
sub-arg-id {A = bind A } =
   begin
     bind (subst-arg (exts ids) A)
   ≡⟨ cong bind (cong-app (cong subst-arg exts-ids) A) ⟩
     bind (subst-arg ids A)
   ≡⟨ cong bind sub-arg-id ⟩
     bind A
   ∎

rename-id : ∀ {Γ} {M : AST Γ} 
  → rename (λ x → x) M ≡ M
rename-id {M = M} =
   begin
     rename (λ x → x) M
   ≡⟨ rename-subst-ren  ⟩
     ⟪ ren (λ x → x) ⟫ M
   ≡⟨⟩
     ⟪ ids ⟫ M
   ≡⟨ sub-id  ⟩
     M
   ∎

sub-idR : ∀{Γ Δ} {σ : Subst Γ Δ}
       → (σ ⨟ ids) ≡ σ
sub-idR {Γ}{σ = σ} =
          begin
            σ ⨟ ids
          ≡⟨⟩
            ⟪ ids ⟫ ∘ σ
          ≡⟨ extensionality (λ x → sub-id) ⟩
            σ
          ∎

compose-ext : ∀{Γ Δ Σ}{ρ : Rename Δ Σ} {ρ′ : Rename Γ Δ}
            → ((ext ρ) ∘ (ext ρ′)) ≡ ext (ρ ∘ ρ′)
compose-ext = extensionality λ x → lemma {x = x}
  where
  lemma : ∀{Γ Δ Σ}{ρ : Rename Δ Σ} {ρ′ : Rename Γ Δ} {x : Var (suc Γ)}
              → ((ext ρ) ∘ (ext ρ′)) x ≡ ext (ρ ∘ ρ′) x
  lemma {x = Z} = refl
  lemma {x = S x} = refl

compose-rename : ∀{Γ Δ Σ}{M : AST Γ}{ρ : Rename Δ Σ}{ρ′ : Rename Γ Δ} 
  → rename ρ (rename ρ′ M) ≡ rename (ρ ∘ ρ′) M
compose-renames : ∀{Γ Δ Σ}{S}{Ms : Args Γ S}{ρ : Rename Δ Σ}{ρ′ : Rename Γ Δ} 
  → renames ρ (renames ρ′ Ms) ≡ renames (ρ ∘ ρ′) Ms
compose-rename-arg : ∀{Γ Δ Σ}{n}{A : Arg Γ n}{ρ : Rename Δ Σ}{ρ′ : Rename Γ Δ} 
  → rename-arg ρ (rename-arg ρ′ A) ≡ rename-arg (ρ ∘ ρ′) A
compose-rename {M = ` x} = refl
compose-rename {M = o ⦅ Ms ⦆} = cong (_⦅_⦆ o) (compose-renames {Ms = Ms})

compose-renames {Ms = nil} = refl
compose-renames {Ms = cons M Ms}{ρ}{ρ′} =
   cong₂ cons compose-rename-arg compose-renames

compose-rename-arg {A = ast M} = cong ast compose-rename
compose-rename-arg {A = bind A}{ρ}{ρ′} =
  let ih = compose-rename-arg {A = A}{ext ρ}{ext ρ′} in
  begin
      bind (rename-arg (ext ρ) (rename-arg (ext ρ′) A))
    ≡⟨ cong bind ih ⟩ 
      bind (rename-arg ((ext ρ) ∘ (ext ρ′)) A) 
    ≡⟨ cong bind (cong₂ rename-arg (compose-ext{ρ = ρ}) refl) ⟩ 
      bind (rename-arg (ext (ρ ∘ ρ′)) A)
    ∎

commute-subst-rename : ∀{Γ Δ}{M : AST Γ}{σ : Subst Γ Δ}
                        {ρ : ∀{Γ} → Rename Γ (suc Γ)}
     → (∀{x : Var Γ} → exts σ (ρ x) ≡ rename ρ (σ x))
     → ⟪ exts σ ⟫ (rename ρ M) ≡ rename ρ (⟪ σ ⟫ M)
commute-subst-rename-arg : ∀{Γ Δ}{n}{A : Arg Γ n}{σ : Subst Γ Δ}
                        {ρ : ∀{Γ} → Rename Γ (suc Γ)}
     → (∀{x : Var Γ} → exts σ (ρ x) ≡ rename ρ (σ x))
     → subst-arg (exts σ) (rename-arg ρ A) ≡ rename-arg ρ (subst-arg σ A)
commute-subst-renames : ∀{Γ Δ}{S}{Ms : Args Γ S}{σ : Subst Γ Δ}
                        {ρ : ∀{Γ} → Rename Γ (suc Γ)}
     → (∀{x : Var Γ} → exts σ (ρ x) ≡ rename ρ (σ x))
     → substs (exts σ) (renames ρ Ms) ≡ renames ρ (substs σ Ms)

commute-subst-rename {M = ` x} r = r
commute-subst-rename {M = o ⦅ Ms ⦆} r =
  cong (_⦅_⦆ o) (commute-subst-renames {Ms = Ms} r)

commute-subst-rename-arg {A = ast M} r =
  cong ast (commute-subst-rename {M = M} r)
commute-subst-rename-arg {Γ}{A = bind A}{σ}{ρ} r =
  let ih = commute-subst-rename-arg {A = A}{exts σ}{ρ′} (λ {x} → H{x}) in
  begin
    bind (subst-arg (exts (exts σ)) (rename-arg (ext ρ) A))
  ≡⟨ cong bind ih ⟩ 
    bind (rename-arg (ext ρ) (subst-arg (exts σ) A))
  ∎
  where
  ρ′ : ∀ {Γ} → Rename Γ (suc Γ)
  ρ′ {zero} = λ ()
  ρ′ {suc Γ} = ext ρ
   
  H : ∀ {x} → exts (exts σ) (ext ρ x) ≡ rename (ext ρ) (exts σ x)
  H {Z} = refl
  H {S y} =
     begin
       exts (exts σ) (ext ρ (S y))
     ≡⟨⟩
       rename S_ (exts σ (ρ y)) 
     ≡⟨ cong (rename S_) r ⟩
       rename S_ (rename ρ (σ y))
     ≡⟨ compose-rename ⟩
       rename (S_ ∘ ρ) (σ y)
     ≡⟨⟩
       rename ((ext ρ) ∘ S_) (σ y)
     ≡⟨ sym compose-rename ⟩
       rename (ext ρ) (rename S_ (σ y))
     ≡⟨⟩
       rename (ext ρ) (exts σ (S y))
     ∎

commute-subst-renames {Ms = nil} r = refl
commute-subst-renames {Γ}{Δ}{_}{cons M Ms}{σ}{ρ} r =
  cong₂ cons (commute-subst-rename-arg{A = M} r)
             (commute-subst-renames{Ms = Ms} r)

exts-seq : ∀{Γ Δ Δ′} {σ₁ : Subst Γ Δ} {σ₂ : Subst Δ Δ′}
         → (exts σ₁ ⨟ exts σ₂) ≡ exts (σ₁ ⨟ σ₂)
exts-seq = extensionality λ x → lemma {x = x}
  where
  lemma : ∀{Γ Δ Δ′}{x : Var (suc Γ)} {σ₁ : Subst Γ Δ}{σ₂ : Subst Δ Δ′}
     → (exts σ₁ ⨟ exts σ₂) x ≡ exts (σ₁ ⨟ σ₂) x
  lemma {x = Z} = refl
  lemma {x = S x}{σ₁}{σ₂} =
     begin
       (exts σ₁ ⨟ exts σ₂) (S x)
     ≡⟨⟩
       ⟪ exts σ₂ ⟫ (rename S_ (σ₁ x))
     ≡⟨ commute-subst-rename{M = σ₁ x}{σ = σ₂}{ρ = S_} refl ⟩
       rename S_ (⟪ σ₂ ⟫ (σ₁ x))
     ≡⟨⟩
       rename S_ ((σ₁ ⨟ σ₂) x)
     ∎

sub-sub : ∀{Γ Δ Σ}{M : AST Γ} {σ₁ : Subst Γ Δ}{σ₂ : Subst Δ Σ} 
            → ⟪ σ₂ ⟫ (⟪ σ₁ ⟫ M) ≡ ⟪ σ₁ ⨟ σ₂ ⟫ M
sub-sub-arg : ∀{Γ Δ Σ}{n}{A : Arg Γ n} {σ₁ : Subst Γ Δ}{σ₂ : Subst Δ Σ} 
            → subst-arg σ₂ (subst-arg σ₁ A) ≡ subst-arg (σ₁ ⨟ σ₂) A
sub-subs : ∀{Γ Δ Σ}{S}{Ms : Args Γ S} {σ₁ : Subst Γ Δ}{σ₂ : Subst Δ Σ} 
            → substs σ₂ (substs σ₁ Ms) ≡ substs (σ₁ ⨟ σ₂) Ms
sub-sub {M = ` x} = refl
sub-sub {M = op ⦅ Ms ⦆} = cong (op ⦅_⦆) (sub-subs{Ms = Ms})

sub-sub-arg {A = ast M} = cong ast (sub-sub {M = M})
sub-sub-arg {A = bind A}{σ₁}{σ₂} =
  let ih = sub-sub-arg {A = A}{exts σ₁}{exts σ₂} in
  begin
    subst-arg σ₂ (subst-arg σ₁ (bind A))
  ≡⟨⟩
    bind (subst-arg (exts σ₂) (subst-arg (exts σ₁) A))
  ≡⟨ cong bind ih ⟩
    bind (subst-arg (exts σ₁ ⨟ exts σ₂) A)
  ≡⟨ cong bind (cong-app (cong subst-arg exts-seq) A) ⟩
    bind (subst-arg (exts (σ₁ ⨟ σ₂)) A)
  ≡⟨⟩
    subst-arg (σ₁ ⨟ σ₂) (bind A)
  ∎

sub-subs {Ms = nil} = refl
sub-subs {Ms = cons M Ms} = cong₂ cons (sub-sub-arg{A = M}) (sub-subs{Ms = Ms})

rename-subst : ∀{Γ Δ Δ′}{M : AST Γ}{ρ : Rename Γ Δ}{σ : Subst Δ Δ′}
             → ⟪ σ ⟫ (rename ρ M) ≡ ⟪ σ ∘ ρ ⟫ M
rename-subst {Γ}{Δ}{Δ′}{M}{ρ}{σ} =
   begin
     ⟪ σ ⟫ (rename ρ M)
   ≡⟨ cong ⟪ σ ⟫ (rename-subst-ren{M = M}) ⟩
     ⟪ σ ⟫ (⟪ ren ρ ⟫ M)
   ≡⟨ sub-sub{M = M} ⟩
     ⟪ ren ρ ⨟ σ ⟫ M
   ≡⟨⟩
     ⟪ σ ∘ ρ ⟫ M
   ∎

sub-assoc : ∀{Γ Δ Σ Ψ} {σ : Subst Γ Δ} {τ : Subst Δ Σ}
             {θ : Subst Σ Ψ}
          → (σ ⨟ τ) ⨟ θ ≡ σ ⨟ τ ⨟ θ
sub-assoc {Γ}{Δ}{Σ}{Ψ}{σ}{τ}{θ} = extensionality λ x → lemma{x = x}
  where
  lemma : ∀ {x : Var Γ} → ((σ ⨟ τ) ⨟ θ) x ≡ (σ ⨟ τ ⨟ θ) x
  lemma {x} =
      begin
        ((σ ⨟ τ) ⨟ θ) x
      ≡⟨⟩
        ⟪ θ ⟫ (⟪ τ ⟫ (σ x))
      ≡⟨ sub-sub{M = σ x} ⟩
        ⟪ τ ⨟ θ ⟫ (σ x)
      ≡⟨⟩
        (σ ⨟ τ ⨟ θ) x
      ∎

subst-zero-exts-cons : ∀{Γ Δ}{σ : Subst Γ Δ}{M : AST Δ}
                     → exts σ ⨟ subst-zero M ≡ M • σ
subst-zero-exts-cons {Γ}{Δ}{σ}{M} =
    begin
      exts σ ⨟ subst-zero M
    ≡⟨ cong₂ _⨟_ exts-cons-shift subst-Z-cons-ids ⟩
      (` Z • (σ ⨟ ↑)) ⨟ (M • ids)
    ≡⟨ sub-dist ⟩
      (⟪ M • ids ⟫ (` Z)) • ((σ ⨟ ↑) ⨟ (M • ids))
    ≡⟨ cong₂ _•_ (sub-head{σ = ids}) refl ⟩
      M • ((σ ⨟ ↑) ⨟ (M • ids))
    ≡⟨ cong₂ _•_ refl (sub-assoc{σ = σ}) ⟩
      M • (σ ⨟ (↑ ⨟ (M • ids)))
    ≡⟨ cong₂ _•_ refl (cong₂ _⨟_ {x = σ} refl (sub-tail{M = M}{σ = ids})) ⟩
      M • (σ ⨟ ids)
    ≡⟨ cong₂ _•_ refl (sub-idR{σ = σ}) ⟩
      M • σ
    ∎

subst-commute : ∀{Γ Δ : ℕ}{N : AST (suc Γ)}{M : AST Γ}{σ : Subst Γ Δ }
    → (⟪ exts σ ⟫ N) [ ⟪ σ ⟫ M ] ≡ ⟪ σ ⟫ (N [ M ])
subst-commute {Γ}{Δ}{N}{M}{σ} =
     begin
       ⟪ exts σ ⟫ N [ ⟪ σ ⟫ M ]
     ≡⟨⟩
       ⟪ subst-zero (⟪ σ ⟫ M) ⟫ (⟪ exts σ ⟫ N)
     ≡⟨ cong-app (cong ⟪_⟫ subst-Z-cons-ids) (⟪ exts σ ⟫ N) ⟩
       ⟪ ⟪ σ ⟫ M • ids ⟫ (⟪ exts σ ⟫ N)
     ≡⟨ sub-sub {M = N} ⟩
       ⟪ (exts σ) ⨟ ((⟪ σ ⟫ M) • ids) ⟫ N
     ≡⟨ cong-app (cong ⟪_⟫ (cong₂ _⨟_ exts-cons-shift refl)) N ⟩
       ⟪ (` Z • (σ ⨟ ↑)) ⨟ (⟪ σ ⟫ M • ids) ⟫ N
     ≡⟨ cong-app (cong ⟪_⟫ (sub-dist {M = ` Z})) N ⟩
       ⟪ ⟪ ⟪ σ ⟫ M • ids ⟫ (` Z) • ((σ ⨟ ↑) ⨟ (⟪ σ ⟫ M • ids)) ⟫ N
     ≡⟨⟩
       ⟪ ⟪ σ ⟫ M • ((σ ⨟ ↑) ⨟ (⟪ σ ⟫ M • ids)) ⟫ N
     ≡⟨ cong-app (cong ⟪_⟫ (cong₂ _•_ refl (sub-assoc{σ = σ}))) N ⟩
       ⟪ ⟪ σ ⟫ M • (σ ⨟ ↑ ⨟ ⟪ σ ⟫ M • ids) ⟫ N
     ≡⟨ refl ⟩
       ⟪ ⟪ σ ⟫ M • (σ ⨟ ids) ⟫ N
     ≡⟨ cong-app (cong ⟪_⟫ (cong₂ _•_ refl (sub-idR{σ = σ}))) N ⟩
       ⟪ ⟪ σ ⟫ M • σ ⟫ N
     ≡⟨ cong-app (cong ⟪_⟫ (cong₂ _•_ refl (sub-idL{σ = σ}))) N ⟩
       ⟪ ⟪ σ ⟫ M • (ids ⨟ σ) ⟫ N
     ≡⟨ cong-app (cong ⟪_⟫ (sym sub-dist)) N ⟩
       ⟪ M • ids ⨟ σ ⟫ N
     ≡⟨ sym (sub-sub{M = N}) ⟩
       ⟪ σ ⟫ (⟪ M • ids ⟫ N)
     ≡⟨ cong ⟪ σ ⟫ (sym (cong-app (cong ⟪_⟫ subst-Z-cons-ids) N)) ⟩
       ⟪ σ ⟫ (N [ M ])
     ∎

rename-subst-commute : ∀{Γ Δ}{N : AST (suc Γ)}{M : AST Γ}{ρ : Rename Γ Δ }
    → (rename (ext ρ) N) [ rename ρ M ] ≡ rename ρ (N [ M ])
rename-subst-commute {Γ}{Δ}{N}{M}{ρ} =
     begin
       (rename (ext ρ) N) [ rename ρ M ]
     ≡⟨ cong-app (cong ⟪_⟫ (cong subst-zero rename-subst-ren)) (rename (ext ρ) N) ⟩
       (rename (ext ρ) N) [ ⟪ ren ρ ⟫ M ]
     ≡⟨ cong ⟪ subst-zero (⟪ ren ρ ⟫ M) ⟫ (rename-subst-ren{M = N}) ⟩
       (⟪ ren (ext ρ) ⟫ N) [ ⟪ ren ρ ⟫ M ]
     ≡⟨  cong ⟪ subst-zero (⟪ ren ρ ⟫ M) ⟫ ( cong-app (cong ⟪_⟫ ren-ext) N) ⟩
       (⟪ exts (ren ρ) ⟫ N) [ ⟪ ren ρ ⟫ M ]
     ≡⟨ subst-commute{N = N} ⟩
       ⟪ ren ρ ⟫ (N [ M ])
     ≡⟨ sym rename-subst-ren ⟩
       rename ρ (N [ M ])
     ∎

_〔_〕 : ∀ {Γ}
        → AST (suc (suc Γ))
        → AST Γ
          ------------
        → AST (suc Γ)
_〔_〕 {Γ} N M = ⟪ exts (subst-zero M) ⟫ N

substitution : ∀{Γ}{M : AST (suc (suc Γ))}{N : AST (suc Γ)}{L : AST Γ}
    → (M [ N ]) [ L ] ≡ (M 〔 L 〕) [ (N [ L ]) ]
substitution{M = M}{N = N}{L = L} =
   sym (subst-commute{N = M}{M = N}{σ = subst-zero L})


data CArgs : (Γ : ℕ) → (Δ : ℕ) → (sig : List ℕ) → Set

data Ctx : ℕ → ℕ → Set where
  CHole : ∀ {Γ} → Ctx Γ Γ
  COp : ∀ {Γ Δ} → (op : Op) → CArgs Γ Δ (sig op) → Ctx Γ Δ

data CArg : (Γ : ℕ) → (Δ : ℕ) → (n : ℕ) → Set where
  CAst : ∀{Γ Δ} → Ctx Γ Δ → CArg Γ Δ 0
  CBind : ∀{Γ Δ}{n} → CArg (suc Γ) (suc Δ) n → CArg (suc Γ) Δ (suc n)

data CArgs where
  tcons : ∀{Γ Δ}{n}{bs bs'} → Arg Δ n → CArgs Γ Δ bs → bs' ≡ (n ∷ bs)
        → CArgs Γ Δ bs'
  ccons : ∀{Γ Δ}{n}{bs bs'} → CArg Γ Δ n → Args Δ bs → bs' ≡ (n ∷ bs)
        → CArgs Γ Δ bs'  

cargs-not-empty : ∀ {Γ Δ} → ¬ CArgs Γ Δ []
cargs-not-empty {Γ} {Δ} (tcons (ast x) Cs ())
cargs-not-empty {Γ} {Δ} (tcons (bind x) Cs ())
cargs-not-empty {Γ} {Δ} (ccons (CAst x) x₁ ())
cargs-not-empty {.(suc _)} {Δ} (ccons (CBind x) x₁ ())

plug : ∀ {Γ Δ} → Ctx Γ Δ → AST Γ → AST Δ
plug-arg : ∀ {Γ Δ n} → CArg Γ Δ n → AST Γ → Arg Δ n
plug-args : ∀ {Γ Δ bs} → CArgs Γ Δ bs → AST Γ → Args Δ bs

plug CHole M = M
plug (COp op args) M = op ⦅ plug-args args M ⦆

plug-arg (CAst C) M = ast (plug C M)
plug-arg (CBind C) M = bind (plug-arg C M)

plug-args (tcons L Cs eq) M rewrite eq =
   cons L (plug-args Cs M)
plug-args (ccons C Ls eq) M rewrite eq =
   cons (plug-arg C M) Ls

